Almost done with proving insertion

Assignment Binary Trees.v
@@ -5,6 +5,11 @@
 
 (* Libraries to import *)
 Require Import Lia.
+Require Import Arith.
+Require Import Bool.
+
+(* Notations *)
+Notation "a >=? b" := (Nat.leb b a) (at level 70) : nat_scope. (* Issue with Nat not defining this? *)
 
 (* Define a tree type *)
 Inductive tree : Set :=
@@ -53,15 +58,19 @@ Definition valid_bst_tree : Prop :=
 
 Theorem is_not_bst_tree : ~invalid_bst_tree.
 Proof.
-unfold invalid_bst_tree.
-simpl.
-lia.
+  unfold invalid_bst_tree.
+  simpl.
+  unfold not; intros.
+  destruct H as [H1 H2].
+  destruct H1 as [H11 H12].
+  lia. (* Solves the fact that 6 < 4 is False *)
 Qed.
 
 Theorem is_bst_tree : valid_bst_tree.
-unfold valid_bst_tree.
-simpl.
-lia.
+Proof.
+  unfold valid_bst_tree.
+  simpl.
+  lia. (* Similar to above *)
 Qed.
 
 End verify_bst_invariant.
@@ -72,13 +81,102 @@ End verify_bst_invariant.
   in the tree.
   So that the insertion does not break the binary search tree
   property.
+  Then return the tree.
 *)
-Fixpoint insert (N : nat) (T : tree ) : tree :=
+Fixpoint insert (N : nat) (T : tree) : tree :=
   match T with
-  | 
+  | leaf => node leaf N leaf
+  | node l n r => if (N <? n) then node (insert N l) n r else if (N >=? n) then node l n (insert N r) else node l n r
   end.
 
+(* Let us prove the correctness of our insert function *)
+Section verify_insert.
 
+Definition test_type : tree :=
+  node (node leaf 4 leaf) 6 (node leaf 10 leaf).
+
+(* A test to confirm our intuition *)
+Theorem insert_test : (insert 4 (insert 10 (insert 6 (leaf)))) = test_type.
+Proof.
+  simpl.
+  unfold test_type.
+  auto.
+Qed.
+
+(*
+  In order to prove that insert behaves correctly for any
+  tree T and node value n, we have to unfold the definition
+  for the inductive propositons defined above. 
+  In order to prove these structures, we need a way to relate
+  a propositon to a boolean.
+  Let us define a function that does this for us, using the
+  Reflection library in Coq.Bool.
+
+  Note: Since we are mainly interested in the less than (<)
+  operator, as defined in our insert function, we shall write
+  the corresponding reflection function.
+*)
+Lemma ltb_reflect : forall x y, reflect (x < y) (x <? y).
+Proof.
+  intros.
+  apply iff_reflect. (* Convert reflect to its value *)
+  symmetry.
+  apply Nat.ltb_lt. (* Lemma to solve the goal - Defined in Arith *)
+Qed.
+
+(* 
+  For our formal proof we also need another theorem. This theorem
+  states that insert should preserve any predicate P on a node,
+  similar to the one we defined for inductively checking the bst
+  property.
+  In summary; for every predicate P and tree T we check that if the
+  bst property holds on P and T, then it should hold on all subsequent
+  subnodes below the starting node T.
+*)
+Theorem bst_prop_insert : forall (P : nat -> tree -> Prop) (T : tree),
+     bst_prop P T -> forall (n : nat) (t : tree),
+     P n t -> bst_prop P (insert n T).
+Proof.
+  intros P T.
+  induction T.
+  intros H1 n t H2.
+  simpl.
+  unfold bst_prop.
+  simpl.
+  simpl. 
+
+  
+  intros.
+  simpl.
+
+(* Let us now formally prove the validity of the insert function *)
+Theorem insert_correct : forall (T : tree) (N : nat), bst T -> bst (insert N T).
+Proof.
+  (* Apply induction and prove the base case *)
+  intros T N.
+  induction T.
+  intros.
+  simpl; auto.
+
+  (* Now prove the step case *)
+  intros.
+  inversion H. (* To discover the cases which must be true for this to hold *)
+  destruct H1 as [H1 H2].
+  destruct H2 as [H2 H3].
+  simpl.
+  destruct (ltb_reflect N n). (* Use the reflection function defined above *)
+  simpl.
+  split.
+  
+  
+  
+  
+
+
+
+
+
+End verify_insert.
 
 
 
